proof/spec/Properties.ec
@@ -21,89 +21,57 @@ lemma set_layer_addr_op_impl (addr : adrs, layer : int):
     set_layer_addr_pre layer => 
         hoare[M(Syscall).__set_layer_addr : 
             arg = (addr, W32.of_int layer) ==> res = set_layer_addr addr layer].
-proof. 
-move => ?. 
-proc. 
-auto. 
-qed.
+proof. move => ?. proc. auto. qed.
 
 lemma set_tree_addr_op_impl (address : adrs, tree_address : int):
     set_tree_addr_pre tree_address => 
         hoare[M(Syscall).__set_tree_addr : 
             arg = (address, W64.of_int tree_address) ==> res = set_tree_addr address tree_address].
-proof. 
-move => ?. 
-proc. 
-auto. 
-qed.
+proof. move => ?. proc. auto. qed.
 
 lemma set_type_op_impl (address : adrs, _type : int):
     set_type_pre _type =>
         hoare[M(Syscall).__set_type :
             arg = (address, W32.of_int _type) ==> res = set_type address _type].
-proof. 
-move => ?.
-proc. 
-auto. 
-qed.
+proof. move => ?. proc. auto. qed.
 
 lemma set_ots_addr_op_impl (address : adrs, ots_addr : int):
     set_ots_addr_pre ots_addr => 
         hoare[M(Syscall).__set_ots_addr :
             arg = (address, W32.of_int ots_addr) ==> res = set_ots_addr address ots_addr].
-proof. 
-move => ?. 
-proc. 
-auto. 
-qed.
+proof. move => ?. proc. auto. qed.
 
 lemma set_chain_addr_op_impl (address : adrs, chain_addr : int):
     set_chain_addr_pre chain_addr => 
         hoare[M(Syscall).__set_chain_addr :
             arg = (address, W32.of_int chain_addr) ==> res = set_chain_addr address chain_addr].
-proof. 
-move => ?. 
-proc. 
-auto. 
-qed.
+proof. move => ?. proc. auto. qed.
 
 lemma set_hash_addr_op_impl (address : adrs, hash_addr : int):
     set_hash_addr_pre hash_addr =>
         hoare[M(Syscall).__set_hash_addr :
             arg = (address, W32.of_int hash_addr) ==> res = set_hash_addr address hash_addr].
-proof. 
-move => ?. 
-proc. 
-auto. 
-qed.
+proof. move => ?. proc. auto. qed.
 
 lemma set_ltree_addr_op_impl (address : adrs, ltree_addr : int):
     set_ltree_addr_pre ltree_addr =>
         hoare[M(Syscall).__set_ltree_addr :
             arg = (address, W32.of_int ltree_addr) ==> 
                 res = set_ltree_addr address ltree_addr].
-proof. 
-move => ?. 
-proc. 
-auto. 
-qed.
+proof. move => ?. proc. auto. qed.
 
 lemma set_tree_height_op_impl (address : adrs, tree_height : int):
     tree_height_pre tree_height =>
         hoare[M(Syscall).__set_tree_height :
             arg = (address, W32.of_int tree_height) ==> res = set_tree_height address tree_height].
-proof. 
-move => ?. 
-proc. 
-auto. 
-qed.
+proof. move => ?. proc. auto. qed.
 
 lemma get_set_tree_height (address : adrs, tree_height : int) :
     tree_height_pre tree_height => 
     get_tree_height (set_tree_height address tree_height) = tree_height.
 proof.
-rewrite /get_tree_height /set_tree_height.
-progress.
+rewrite /get_tree_height /set_tree_height /tree_height_pre.
+move => ?.
 smt.
 qed.
 
@@ -111,30 +79,20 @@ lemma set_tree_index_op_impl (address : adrs, tree_index) :
     set_tree_index_pre tree_index => 
         hoare[M(Syscall).__set_tree_index :
             arg = (address, W32.of_int tree_index) ==> res = set_tree_index address tree_index].
-proof. 
-move => ?. 
-proc. 
-auto. 
-qed.
+proof. move => ?. proc. auto. qed.
 
 lemma get_set_tree_index (address : adrs, tree_index : int) :
   0 <= tree_index < W32.modulus => (* i.e. tree_index fits in a u32 *)
   get_tree_index (set_tree_index address tree_index) = tree_index.  
-proof.
-rewrite /get_tree_index /set_tree_index.
-progress.
-smt.
-qed.
+proof. rewrite /get_tree_index /set_tree_index. move => ?. smt(get_setE @W32). qed.
 
 lemma set_key_and_mask_op_impl (address : adrs, key_and_mask : int):
     hoare[M(Syscall).__set_key_and_mask :
         arg = (address, W32.of_int key_and_mask) ==> res = set_key_and_mask address key_and_mask].
-proof. 
-proc. 
-auto. 
-qed.
+proof. proc. auto. qed.
 
 op zero_addr : adrs = Array8.init (fun _ => W32.zero). 
+
 lemma zero_addr_op_impl (address : adrs) :
     hoare[M(Syscall)._zero_address : true ==> res = zero_addr].
 proof.
@@ -142,6 +100,15 @@ proc.
 while (0 <= i <= 8 /\ 
       (forall (k : int), 0 <= k < i => (addr.[k] = W32.zero))); auto => /> ; smt(get_setE tP initiE).
 qed.
+
+(******************************************************* THASH_ *******************************************************)
+
+op thash_f (address : adrs, _seed : seed, t : nbytes) : nbytes =
+    let address = set_key_and_mask address 0 in
+    let _key = PRF _seed address in
+    let address = set_key_and_mask address 1 in
+    let bitmask = PRF _seed address in
+    F _key (nbytexor t bitmask).
 
 (***************************************************** PRIMITIVES *****************************************************)
 
@@ -189,20 +156,18 @@ qed.
 
 module Checksum = {
   (* part of WOTS *)
-  proc checksum (m : nbytes) : W32.t = {
+  proc checksum (m : W32.t list) : W32.t = {
     var i : int <- 0;
-    var m_i : W8.t <- witness;
-    var checksum : W32.t <- W32.zero;
+    var m_i : W32.t <- witness;
+    var checksum : int <- 0;
 
     while (i < len1) {
       m_i <- nth witness m i;
-      checksum <- checksum + W32.of_int(w - 1) - (W32_of_W8 m_i);
+      checksum <- checksum + (w - 1) - (W32.to_uint m_i);
       i <- i + 1;
     }
 
-    checksum <- checksum `<<` W8.of_int (8 - ((ceil (len2%r * log2(w%r))) %% 8));
-
-    return checksum;
+    return (W32.of_int checksum);
   }
 }.
 
